Document `modsp`

src/sem/ModSP.v
@@ -1,20 +1,56 @@
 Require SemanticCommon.
 
 Import MemoryOps Instruction State SemanticCommon.
-(**
+(**  
 <<
-## ModSP
+# ModSP
+
+## Syntax
+
+```
+OpModSP in1, out1
+```
+
+## Summary
+
+Ignores its operands but adjusts SP if `RelSpPop` and/or `RelSPPush` modes are
+used.
 
 >>
-Performs no operations with memory, but may adjust SP using address modes
-[RelSpPop] and [RelSPPush].
+See [Arg.RelSpPush], [Arg.RelSpPop].
+
+<<
+## Semantic
+
+- Advances PC
+- May modify SP if `in` uses `RelSpPop` addressing mode, or `out` uses
+  `RelSpPush` mode. Both operands may affect SP simultaneously; the general
+  rules apply, so first `in` will affect SP, then `out` will affect SP.
+
+## Affected parts of VM state
+
+- execution stack : PC is increased; SP may be changed.
+
+## Usage
+
+The primary use is adjusting SP.
+
+## Similar instructions
+
+- If `in` does not use `RelSpPop` and `out` does not use `RelSpPush`, this instruction does nothing, like `NoOp`.
+
+## Encoding
+
+- `ModSP` and `NoOp` have the same encoding.
+
+>>
 *)
 
 Inductive step : instruction -> smallstep :=
 | step_ModSP:
   forall codes flags depot pages xstack0 xstack1 new_xstack context_u128 in1 out1 regs,
-    resolve_effect__in in1 xstack0 xstack1 ->
-    resolve_effect__out out1 xstack1 new_xstack ->
+    resolve_effect__in in1 xstack0 xstack1 ->      (* Account for possible [RelSpPop]. *)
+    resolve_effect__out out1 xstack1 new_xstack ->(* Account for possible [RelSpPush]. *)
     step (OpModSP in1 out1)
           {|
           gs_callstack    := xstack0;
@@ -39,3 +75,72 @@ Inductive step : instruction -> smallstep :=
           gs_contracts    := codes;
           |}
 .
+
+(**
+<<
+## Examples
+
+>>
+
+ *)
+Section Examples.
+Import Arg Arg.Coercions ZMod Memory ZArith ExecutionStack.
+Open Scope Z.
+Coercion int_mod_of : Z >-> int_mod.
+Set Printing Coercions.
+
+(**
+<<
+`modsp stack-=[23], stack+=[88]`
+>>
+*)
+
+Section Ex1.
+Let ex := OpModSP (RelSpPop R0 23) (RelSpPush R0 88) : instruction.
+(* Import ZMod.
+Goal 
+  forall codes flags depot pages xstack0 context_u128 regs,
+    step ex 
+          {|
+          gs_callstack    := xstack0;
+          gs_flags        := flags;
+          gs_regs         := regs;
+          gs_pages        := pages;
+          gs_depot        := depot;
+          gs_context_u128 := context_u128;
+          gs_contracts    := codes;
+          |}
+          {|
+          gs_callstack    := ExecutionStack.sp_mod  (fun sp =>
+                                                       fst ((fst (sp + 23)) - 88 )) xstack0;
+
+
+          gs_flags        := flags;
+          gs_regs         := regs;
+          gs_pages        := pages;
+          gs_depot        := depot;
+          gs_context_u128 := context_u128;
+          gs_contracts    := codes;
+          |}
+.
+  Proof.
+    intros codes flags depot pages xstack0 context_u128 regs.
+    apply step_ModSP with (xstack1 := ExecutionStack.sp_mod (fun sp => fst (sp + 23)) xstack0); simpl.
+    - destruct xstack0.
+      + simpl.
+        destruct c.
+        simpl.
+        unfold RecordSet.set.
+simpl.
+        econstructor 1 with (regs := regs) (arg := RelSpPop R0 23).
+        * econstructor ; eauto.
+          econstructor; eauto.
+          constructor.
+          constructor.
+          constructor.
+          simpl.
+          reflexivity.
+    *)
+Fail Check OpModSP (RelSpPush R1 23) (RelSpPush R3 88) : instruction.
+End Ex1.
+End Examples.
